theories/FV.v
@@ -5,27 +5,32 @@ Definition set A := A -> Prop.
 
 Definition empty_set {A} : set A :=
   fun _ => False.
+Arguments empty_set {A}/ x.
 
-Definition singleton_set {A} (x : A) : set A :=
-  fun y => x = y.
+Definition singleton_set {A} (e : A) : set A :=
+  fun x => e = x.
+Arguments singleton_set {A} e/ x.
 
 Definition set_union {A} (X Y : set A) : set A :=
   fun x => X x \/ Y x.
+Arguments set_union {A} X Y/ x.
 
 Definition set_intersection {A} (X Y : set A) : set A :=
   fun x => X x /\ Y x.
+Arguments set_intersection {A} X Y/ x.
 
 Definition set_minus {A} (X Y : set A) : set A :=
   fun x => X x /\ ~(Y x).
+Arguments set_minus {A} X Y/ x.
 
 Definition Disjoint {A} (X Y : set A) : Prop :=
   (forall x, X x -> ~(Y x)) /\ (forall x, Y x -> ~(X x)).
 
 (* Meant to be read with *currying* in mind: `Contains a b` = `(Contains a) b`, i.e. "b contains a" *)
-Definition Contains {T} (a b : set T) := forall x, a x -> b x.
+Definition Contains {T} (a b : set T) : Prop := forall x, a x -> b x.
 Arguments Contains/ {T} a b.
 
-Definition SetEq {T} (a b : set T) := forall x, a x <-> b x.
+Definition SetEq {T} (a b : set T) : Prop := forall x, a x <-> b x.
 Arguments SetEq/ {T} a b.
 
 Class FV (A : Type) := { fv : A -> set ident }.
