theories/Semantics.v
@@ -11,7 +11,7 @@ Inductive Step : env -> term -> term -> prefix -> Prop :=
   | S_One_R : forall n,
       Step n unit sink PfxOneFull
   | S_Var : forall n x p,
-      MapsTo p x n ->
+      n x = Some p ->
       Step n (TmVar x) (TmVar x) p
   | S_Par_R : forall n e1 e1' e2 e2' p1 p2,
       Step n e1 e1' p1 ->
@@ -27,11 +27,11 @@ Inductive Step : env -> term -> term -> prefix -> Prop :=
       Step n e2 e2' p2 ->
       Step n (e1; e2) e2' (PfxCatBoth p1 p2)
   | S_Par_L : forall n x y z e e' p1 p2 p',
-      MapsTo (PfxParPair p1 p2) z n ->
+      n z = Some (PfxParPair p1 p2) ->
       Step (env_union n (env_union (singleton_env x p1) (singleton_env y p2))) e e' p' ->
       Step n (TmLetPar x y z e) (TmLetPar x y z e') p'
   | S_Cat_L_1 : forall t n x y z e e' p p',
-      MapsTo (PfxCatFst p) z n ->
+      n z = Some (PfxCatFst p) ->
       Step (subst x p (subst y (emp t) n)) e e' p' ->
       Step n (TmLetCat t x y z e) (TmLetCat t x y z e') p'
   .
